Some refactoring

fairneris/examples/retransmit_model.v
@@ -6,6 +6,145 @@ From fairneris.aneris_lang Require Import ast network.
 
 Import derived_laws_later.bi.
 
+(* Trace Utils - TODO: Move to trace_utils.v *)
+Fixpoint trace_take {S L} (n : nat) (tr : trace S L) : finite_trace S L :=
+  match tr with
+  | ⟨s⟩ => {tr[s]}
+  | s -[ℓ]-> r => match n with
+                  | 0 => {tr[s]}
+                  | S n => (trace_take n r) :tr[ℓ]: s
+                  end
+  end.
+
+Fixpoint trace_filter {S L} (f : S → L → Prop)
+           `{∀ s l, Decision (f s l)}
+           (tr : finite_trace S L) : finite_trace S L :=
+  match tr with
+  | {tr[s]} => {tr[s]}
+  | tr :tr[ℓ]: s => if (bool_decide (f s ℓ))
+                    then trace_filter f tr :tr[ℓ]: s
+                    else trace_filter f tr
+  end.
+
+Fixpoint count_labels {S L} (ft : finite_trace S L) : nat :=
+  match ft with
+  | {tr[_]} => 0
+  | ft' :tr[_]: _ => Datatypes.S (count_labels ft')
+  end.
+
+Lemma count_labels_sum {S L} (P : S → L → Prop)
+           `{∀ s l, Decision (P s l)} n m mtr mtr' :
+  after n mtr = Some mtr' →
+  count_labels (trace_filter P $ trace_take (n+m) mtr) =
+  count_labels ((trace_filter P $ trace_take n mtr)) +
+    count_labels ((trace_filter P $ trace_take m mtr')).
+Proof.
+  revert mtr mtr'.
+  induction n=> /=; intros mtr mtr' Hafter.
+  { simplify_eq. by destruct mtr'. }
+  destruct mtr; [done|]. simpl.
+  case_bool_decide.
+  - simpl. f_equiv. by apply IHn.
+  - by apply IHn.
+Qed.
+
+Lemma pred_at_impl {S L} (tr:trace S L) n (P Q : S → option L → Prop) :
+  (∀ s l, P s l → Q s l) → pred_at tr n P → pred_at tr n Q.
+Proof.
+  rewrite /pred_at. intros HPQ HP.
+  destruct (after n tr); [|done].
+  by destruct t; apply HPQ.
+Qed.
+
+Lemma pred_at_neg {S L} (tr:trace S L) n (P : S → option L → Prop) :
+  is_Some (after n tr) →
+  ¬ pred_at tr n P ↔ pred_at tr n (λ s l, ¬ P s l).
+Proof.
+  rewrite /pred_at. intros Hafter. split.
+  - intros HP.
+    destruct (after n tr).
+    + by destruct t.
+    + by apply is_Some_None in Hafter.
+  - intros HP.
+    destruct (after n tr).
+    + by destruct t.
+    + by apply is_Some_None in Hafter.
+Qed.
+
+Lemma infinite_trace_after' {S T} n (tr : trace S T) :
+  infinite_trace tr -> ∃ tr', after n tr = Some tr' ∧ infinite_trace tr'.
+Proof. 
+  revert tr.
+  induction n; intros tr Hinf.
+  { exists tr. done. }
+  pose proof (IHn _ Hinf) as [tr' [Hafter Hinf']].
+  pose proof (Hinf' 1) as [tr'' Htr'].
+  exists tr''.
+  replace (Datatypes.S n) with (n + 1) by lia.
+  rewrite after_sum'. rewrite Hafter. split; [done|].
+  intros n'.
+  specialize (Hinf' (Datatypes.S n')).
+  destruct tr'; [done|].
+  simpl in *. simplify_eq. done.
+Qed.
+
+
+Fixpoint finite_trace_to_trace {S L} (tr : finite_trace S L) : trace S L :=
+  match tr with
+  | {tr[s]} => ⟨s⟩
+  | tr :tr[ℓ]: s => s -[ℓ]-> (finite_trace_to_trace tr)
+  end.
+
+Definition trace_now {S T} (tr : trace S T) P := pred_at tr 0 P.
+Definition trace_always {S T} (tr : trace S T) P := ∀ n, pred_at tr n P.
+Definition trace_eventually {S T} (tr : trace S T) P := ∃ n, pred_at tr n P.
+Definition trace_until {S T} (tr : trace S T) P Q :=
+  ∃ n, pred_at tr n Q ∧ ∀ m, m < n → pred_at tr m P.
+
+Lemma pred_at_after_is_Some {S T} (tr : trace S T) n P :
+  pred_at tr n P → is_Some $ after n tr.
+Proof. rewrite /pred_at. by case_match. Qed.
+
+Lemma after_is_Some_le {S T} (tr : trace S T) n m :
+  m ≤ n → is_Some $ after n tr → is_Some $ after m tr.
+Proof.
+  revert tr m.
+  induction n; intros tr m Hle.
+  { intros. assert (m = 0) as -> by lia. done. }
+  intros.
+  destruct m; [done|].
+  simpl in *.
+  destruct tr; [done|].
+  apply IHn. lia. done.
+Qed.
+
+Lemma trace_eventually_until {S T} (tr : trace S T) P :
+  trace_eventually tr P → trace_until tr (λ s l, ¬ P s l) P.
+Proof.
+  intros [n Hn].
+  induction n as [n IHn] using lt_wf_ind.
+  assert ((∀ m, m < n → pred_at tr m (λ s l, ¬ P s l)) ∨
+            ¬ (∀ m, m < n → pred_at tr m (λ s l, ¬ P s l))) as [HP|HP];
+    [|by eexists _|].
+  { apply ExcludedMiddle. }
+  eapply not_forall_exists_not in HP as [n' HP].
+  apply Classical_Prop.imply_to_and in HP as [Hlt HP].
+  apply pred_at_neg in HP; last first.
+  { eapply after_is_Some_le; [|by eapply pred_at_after_is_Some]. lia. }
+  eapply pred_at_impl in HP; last first.
+  { intros s l H. apply NNP_P. apply H. }
+  specialize (IHn n' Hlt HP) as [n'' [H' H'']].
+  exists n''. done.
+Qed.
+
+Lemma prefix_trans {A} (l1 l2 l3 : list A) :
+  l1 `prefix_of` l2 → l2 `prefix_of` l3 → l1 `prefix_of` l3.
+Proof. intros [l1' ->] [l2' ->]. by do 2 apply prefix_app_r. Qed.
+
+Lemma suffix_trans {A} (l1 l2 l3 : list A) :
+  l1 `suffix_of` l2 → l2 `suffix_of` l3 → l1 `suffix_of` l3.
+Proof. intros [l1' ->] [l2' ->]. by do 2 apply suffix_app_r. Qed.
+
 (** The retransmit model states *)
 Inductive retransmit_base_state :=
 | Start
@@ -68,11 +207,9 @@ Qed.
 
 Definition saA : socket_address := SocketAddressInet "0.0.0.0" 80.
 Definition saB : socket_address := SocketAddressInet "0.0.0.1" 80.
-Definition mAB : message :=
-  mkMessage saA saB "Hello".
+Definition mAB : message := mkMessage saA saB "Hello".
 
-Inductive retransmit_trans
-  : retransmit_state → retransmit_label → retransmit_state → Prop :=
+Inductive retransmit_trans : retransmit_state → retransmit_label → retransmit_state → Prop :=
 | A_Send st ms bs :
   retransmit_trans (st, ms, bs)
                    (inl $ (Arole, Some mAB))
@@ -104,25 +241,6 @@ Inductive retransmit_trans
                    (inl $ (Brole, None))
                    (Received, ms, <[saB := ms']>bs).
 
-Fixpoint trace_take {S L} (n : nat) (tr : trace S L) : finite_trace S L :=
-  match tr with
-  | ⟨s⟩ => {tr[s]}
-  | s -[ℓ]-> r => match n with
-                  | 0 => {tr[s]}
-                  | S n => (trace_take n r) :tr[ℓ]: s
-                  end
-  end.
-
-Fixpoint trace_filter {S L} (f : S → L → Prop)
-           `{∀ s l, Decision (f s l)}
-           (tr : finite_trace S L) : finite_trace S L :=
-  match tr with
-  | {tr[s]} => {tr[s]}
-  | tr :tr[ℓ]: s => if (bool_decide (f s ℓ))
-                    then trace_filter f tr :tr[ℓ]: s
-                    else trace_filter f tr
-  end.
-
 Definition send_filter msg : retransmit_state → retransmit_label → Prop :=
   λ _ l, ∃ r, l = inl (r,Some(msg)).
 Instance send_filter_decision msg st l : Decision (send_filter msg st l).
@@ -136,21 +254,16 @@ Proof. apply make_decision. Qed.
 Class Monotone (f : nat → nat) :=
   { mono_incr : ∀ n m, n ≤ m → f n ≤ f m; }.
 
-Fixpoint count_labels {S L} (ft : finite_trace S L) : nat :=
-  match ft with
-  | {tr[_]} => 0
-  | ft' :tr[_]: _ => Datatypes.S (count_labels ft')
-  end.
-
 Definition count_sends (msg : message) tr : nat :=
   count_labels (trace_filter (send_filter msg) tr).
 
 Definition count_delivers (msg : message) tr : nat :=
   count_labels (trace_filter (deliver_filter msg) tr).
 
-Definition retransmit_network_fair_delivery
-           (tr:trace retransmit_state retransmit_label) : Prop :=
-  ∃ f1 f2 `{Monotone f1} `{Monotone f2},
+Notation mtrace := (trace retransmit_state retransmit_label).
+
+Definition retransmit_network_fair_delivery (tr : mtrace) : Prop :=
+  ∃ (f1 f2 : nat → nat) `(Monotone f1) `(Monotone f2),
     ∀ msg n,
       let sends := count_sends msg (trace_take n tr) in
       let delivers := count_delivers msg (trace_take n tr) in
@@ -163,46 +276,27 @@ Definition retransmit_live_roles (s : retransmit_state) : gset retransmit_role :
    else {[inr Ndup;inr Ndrop;inr Ndeliver]}) ∪
   (match s.1.1 with Start => {[inl Brole]} | _ => ∅ end).
 
-(* TODO: We might need this later *)
-(* Lemma retransmit_live_spec_holds s ρ s' : *)
-(*   retransmit_trans s ρ s' → label_role ρ ∈ retransmit_live_roles s. *)
-(* Proof. Admitted. *)
-
 (* TODO: This should be generalised, and lifted to multiple roles *)
-Definition retransmit_terminating_role
-           (ρ : retransmit_role)
-           (tr : trace retransmit_state retransmit_label)
-  : Prop :=
+Definition retransmit_terminating_role (ρ : retransmit_role) (tr : mtrace) : Prop :=
   ∃ n, after n tr = None ∨ pred_at tr n (λ st _, ρ ∉ retransmit_live_roles st).
 
-Definition retransmit_role_enabled_model
-           (ρ : retransmit_role) (s : retransmit_state) :=
+Definition retransmit_role_enabled_model (ρ : retransmit_role) (s : retransmit_state) : Prop :=
   ρ ∈ retransmit_live_roles s.
-
-Notation mtrace := (trace retransmit_state retransmit_label).
 
 Definition retransmit_fair_scheduling_mtr (ρ : retransmit_role) : mtrace → Prop :=
   trace_implies (λ δ _, retransmit_role_enabled_model ρ δ)
                 (λ δ ℓ, ¬ retransmit_role_enabled_model ρ δ ∨
                           option_map label_role ℓ = Some ρ).
 
-Lemma retransmit_fair_scheduling_mtr_after ℓ tr tr' k:
+Lemma retransmit_fair_scheduling_mtr_after ℓ tr tr' k :
   after k tr = Some tr' →
   retransmit_fair_scheduling_mtr ℓ tr → retransmit_fair_scheduling_mtr ℓ tr'.
 Proof. apply trace_implies_after. Qed.
 
-(* Lemma fair_scheduling_mtr_cons ℓ δ ℓ' r: *)
-(*   fair_scheduling_mtr ℓ (δ -[ℓ']-> r) → fair_scheduling_mtr ℓ r. *)
-(* Proof. apply trace_implies_cons. Qed. *)
-
-(* Lemma fair_scheduling_mtr_cons_forall δ ℓ' r: *)
-(*   (∀ ℓ, fair_scheduling_mtr ℓ (δ -[ℓ']-> r)) → (∀ ℓ, fair_scheduling_mtr ℓ r). *)
-(* Proof. intros Hℓ ℓ. eapply trace_implies_cons. apply Hℓ. Qed. *)
-
-Definition retransmit_fair_scheduling mtr :=
+Definition retransmit_fair_scheduling (mtr : mtrace) : Prop :=
   ∀ ρ, retransmit_fair_scheduling_mtr ρ mtr.
 
-Lemma retransmit_fair_scheduling_after tr tr' k:
+Lemma retransmit_fair_scheduling_after tr tr' k :
   after k tr = Some tr' →
   retransmit_fair_scheduling tr → retransmit_fair_scheduling tr'.
 Proof.
@@ -210,13 +304,8 @@ Proof.
   by eapply retransmit_fair_scheduling_mtr_after.
 Qed.
 
-Definition mtrace_fair mtr :=
+Definition mtrace_fair (mtr : mtrace) : Prop :=
   retransmit_fair_scheduling mtr ∧ retransmit_network_fair_delivery mtr.
-
-(* Lemma mtrace_fair_after tr tr' k: *)
-(*   after k tr = Some tr' → *)
-(*   mtrace_fair tr → mtrace_fair tr'. *)
-(* Proof. Admitted. *)
 
 Inductive mtrace_valid_ind (mtrace_valid_coind: mtrace → Prop) :
   mtrace → Prop :=
@@ -247,98 +336,8 @@ Proof.
   by inversion Hval'.
 Qed.
 
-Lemma retransmit_fair_traces_terminate_aux (mtr: mtrace) :
-  (trfirst mtr).1.1 = Received → retransmit_terminating_role (inl Brole) mtr.
-Proof.
-  intros Htrfirst.
-  exists 0. rewrite /pred_at=> /=. simpl in *.
-  destruct mtr as [s|s mtr].
-  - rewrite /pred_at=> /=. simpl in *. destruct s as [[??]?]. simpl in *.
-    simplify_eq. rewrite /retransmit_live_roles. simpl in *.
-    case_decide; set_solver.
-  - rewrite /pred_at=> /=. simpl in *. destruct s as [[??]?]. simpl in *.
-    simplify_eq. rewrite /retransmit_live_roles. simpl in *.
-    case_decide; set_solver.
-Qed.
-
-Lemma pred_at_impl {S L} (tr:trace S L) n (P Q : S → option L → Prop) :
-  (∀ s l, P s l → Q s l) → pred_at tr n P → pred_at tr n Q.
-Proof.
-  rewrite /pred_at. intros HPQ HP.
-  destruct (after n tr); [|done].
-  by destruct t; apply HPQ.
-Qed.
-
-Lemma pred_at_neg {S L} (tr:trace S L) n (P : S → option L → Prop) :
-  is_Some (after n tr) →
-  ¬ pred_at tr n P ↔ pred_at tr n (λ s l, ¬ P s l).
-Proof.
-  rewrite /pred_at. intros Hafter. split.
-  - intros HP.
-    destruct (after n tr).
-    + by destruct t.
-    + by apply is_Some_None in Hafter.
-  - intros HP.
-    destruct (after n tr).
-    + by destruct t.
-    + by apply is_Some_None in Hafter.
-Qed.
-
-(* (* TODO: Might need n < m *) *)
-(* Lemma retransmit_trace_sends_grows msg (mtr : mtrace) n : *)
-(*   (∀ n, is_Some (after n mtr)) →  *)
-(*   mtrace_valid mtr → mtrace_fair mtr → *)
-(*   ∃ m, count_sends msg (trace_take n mtr) < count_sends msg (trace_take m mtr). *)
-(* Proof. Admitted. *)
-
-Lemma count_labels_sum {S L} (P : S → L → Prop)
-           `{∀ s l, Decision (P s l)} n m mtr mtr' :
-  after n mtr = Some mtr' →
-  count_labels (trace_filter P $ trace_take (n+m) mtr) =
-  count_labels ((trace_filter P $ trace_take n mtr)) +
-    count_labels ((trace_filter P $ trace_take m mtr')).
-Proof.
-  revert mtr mtr'.
-  induction n=> /=; intros mtr mtr' Hafter.
-  { simplify_eq. by destruct mtr'. }
-  destruct mtr; [done|]. simpl.
-  case_bool_decide.
-  - simpl. f_equiv. by apply IHn.
-  - by apply IHn.
-Qed.
-
-(* Lemma count_sends_sum msg n m mtr mtr' : *)
-(*   after n mtr = Some mtr' → *)
-(*   count_sends msg (trace_take (n+m) mtr) = *)
-(*   count_sends msg (trace_take n mtr) + count_sends msg (trace_take m mtr'). *)
-(* Proof. Admitted. *)
-
-
-Lemma infinite_trace_after' {S T} n (tr : trace S T) :
-  infinite_trace tr -> ∃ tr', after n tr = Some tr' ∧ infinite_trace tr'.
-Proof. 
-  revert tr.
-  induction n; intros tr Hinf.
-  { exists tr. done. }
-  pose proof (IHn _ Hinf) as [tr' [Hafter Hinf']].
-  pose proof (Hinf' 1) as [tr'' Htr'].
-  exists tr''.
-  replace (Datatypes.S n) with (n + 1) by lia.
-  rewrite after_sum'. rewrite Hafter. split; [done|].
-  intros n'.
-  specialize (Hinf' (Datatypes.S n')).
-  destruct tr'; [done|].
-  simpl in *. simplify_eq. done.
-Qed.
-
-(* TODO: Might need n < m *)
-(* OBS: Not correct - Counting of delivers is incorrect. *)
 Lemma retransmit_trace_delivers_0 (mtr : mtrace) n :
-  (∀ n : nat,
-     pred_at mtr n
-             (λ (_ : retransmit_state) (l : option retransmit_label),
-                l ≠ Some (inr (Ndeliver, mAB)))) →
-  (* mtrace_valid mtr → (* mtrace_fair mtr → *) *)
+  (∀ n : nat, pred_at mtr n (λ _ l, l ≠ Some (inr (Ndeliver, mAB)))) →
   count_delivers mAB (trace_take n mtr) = 0.
 Proof.
   revert mtr.
@@ -359,39 +358,6 @@ Proof.
   - apply IHn.
     intros n'. specialize (Hpred (S n')). rewrite pred_at_S in Hpred. done.
 Qed.
-
-(* (* TODO: Might need n < m *) *)
-(* (* OBS: Not correct - Counting of delivers is incorrect. *) *)
-(* Lemma retransmit_trace_delivers_0 (mtr : mtrace) n : *)
-(*   infinite_trace mtr → *)
-(*   (∀ n : nat, *)
-(*      pred_at mtr n *)
-(*              (λ (_ : retransmit_state) (l : option retransmit_label), *)
-(*                 l ≠ Some (inr (Ndeliver, mAB)))) → *)
-(*   (* mtrace_valid mtr → (* mtrace_fair mtr → *) *) *)
-(*   count_delivers mAB (trace_take n mtr) = 0. *)
-(* Proof. *)
-(*   revert mtr. *)
-(*   induction n; intros mtr Hinf Hpred. *)
-(*   { simpl. specialize (Hpred 0). *)
-(*     destruct mtr; simpl in *. *)
-(*     - rewrite /pred_at in Hpred. simpl in *. *)
-(*       rewrite /count_delivers. done. *)
-(*     - rewrite /pred_at in Hpred. simpl in *. *)
-(*       rewrite /count_delivers. done. *)
-(*   } *)
-(*   simpl in *. *)
-(*   destruct mtr; [done|]. *)
-(*   (* specialize (Hpred (S n)). *) *)
-(*   (* rewrite pred_at_S in Hpred. *) *)
-(*   rewrite /count_delivers. simpl. *)
-(*   case_bool_decide. *)
-(*   - specialize (Hpred 0). rewrite pred_at_0 in Hpred. rewrite /deliver_filter in H. *)
-(*     simplify_eq.  *)
-(*   - apply IHn. *)
-(*     + by eapply infinite_cons. *)
-(*     + intros n'. specialize (Hpred (S n')). rewrite pred_at_S in Hpred. done. *)
-(* Qed. *)
 
 Lemma A_always_live (mtr : mtrace) n :
   infinite_trace mtr →
@@ -449,55 +415,28 @@ Proof.
     exists Arole. done.
 Qed.
 
-(* Lemma pred_at_take n tr tr' : *)
-(*   pred_at tr n = trace_take n $ pred_at tr n.  *)
-(* Lemma trace_take_after n tr tr' : *)
-(*   after n tr = Some tr' → *)
-(*   trace_take n tr = tr'. *)
-
+(* TODO: This can possibly be generalised *)
 Lemma count_sends_pred_at n tr :
-  pred_at tr n (λ (_ : retransmit_state) (l : option retransmit_label),
-            ∃ r : retransmit_node_role,
-              l = Some (inl (r, Some mAB))) →
-  0 < count_labels $ trace_filter (send_filter mAB) (trace_take (S n) tr).
+  pred_at tr n (λ _ l, ∃ r : retransmit_node_role, l = Some (inl (r, Some mAB))) →
+  0 < count_sends mAB (trace_take (S n) tr).
 Proof.
   revert tr.
   induction n=> /=; intros tr Hpred_at.
   { rewrite /pred_at in Hpred_at.    
     destruct tr; simpl in *.
     - destruct Hpred_at as [? ?]. done.
-    - destruct Hpred_at as [? ?].
+    - destruct Hpred_at as [? ?]. rewrite /count_sends=> /=.
       case_bool_decide.
       + simpl. lia.
       + destruct ℓ; [|done]. simplify_eq. rewrite /send_filter in H0.
         eapply not_exists_forall_not in H0. done. }
   simpl in *.
   destruct tr; [done|].
-  simpl in *.
+  simpl in *. rewrite /count_sends=> /=.
   case_bool_decide.
   - simpl. lia.
   - apply IHn. done.
 Qed.
-
-(* Lemma count_labels_pred_at {S L} (P : S → option L → Prop) (Q : S → L → Prop) *)
-(*            `{∀ s l, Decision (Q s l)} n tr : *)
-(*   (∀ s l, P s (Some l) ↔ Q s l) → pred_at tr n P → *)
-(*   0 < count_labels $ trace_filter Q (trace_take n tr). *)
-(* Proof. *)
-  
-(* Admitted. *)
-
-(* Lemma count_sends_pred_at {S L} (P : S → option L → Prop) (Q : S → L → Prop) *)
-(*            `{∀ s l, Decision (Q s l)} n tr : *)
-(*   (∀ s l, P s (Some l) ↔ Q s l) → pred_at tr n P → *)
-(*   0 < count_labels $ trace_filter Q (trace_take n tr). *)
-(* Proof. Admitted. *)
-
-(* Lemma count_sends_pred_at {S L} (P : S → option L → Prop) *)
-(*            `{∀ s l, Decision (P s l)} n tr : *)
-(*   pred_at tr n P → *)
-(*   0 < trace_length $ trace_filter (λ s l, P s (Some l)) (trace_take n tr). *)
-(* Proof. Admitted. *)
 
 (* Any fair infinite trace grow the number of sends indefinitely *)
 Lemma retransmit_trace_sends_grows (mtr : mtrace) x :
@@ -527,37 +466,8 @@ Proof.
   lia.
 Qed.
 
-(* (* Any fair infinite trace grow the number of sends indefinitely *) *)
-(* Lemma retransmit_trace_sends_grows (mtr : mtrace) x : *)
-(*   infinite_trace mtr → *)
-(*   mtrace_valid mtr → retransmit_fair_scheduling mtr → *)
-(*   ∃ n, x < count_sends mAB (trace_take n mtr). *)
-(* Proof. *)
-(*   intros Hafter Hvalid Hfair. *)
-(*   induction x. *)
-(*   { assert (∃ n, pred_at mtr n (λ st l, ∃ r, l = Some $ inl (r,Some mAB))) *)
-(*       as [n Hn]. *)
-(*     { by apply retransmit_fair_traces_eventually_mAB. } *)
-(*     exists n. *)
-(*     eapply count_labels_pred_at; [|done]. rewrite /send_filter. naive_solver. } *)
-(*   destruct IHx as [n IHn]. *)
-(*   apply (infinite_trace_after' n) in Hafter as (mtr' & Hmtr' & Hafter). *)
-(*   assert (∃ n, pred_at mtr' n (λ st l, ∃ r, l = Some $ inl (r,Some mAB))) *)
-(*     as [m Hm]. *)
-(*   { apply retransmit_fair_traces_eventually_mAB; *)
-(*       [done|by eapply mtrace_valid_after| *)
-(*         by eapply retransmit_fair_scheduling_after]. } *)
-(*   assert (0 < count_sends mAB (trace_take m mtr')). *)
-(*   { eapply count_labels_pred_at; [|done]. *)
-(*     rewrite /send_filter. naive_solver. } *)
-(*   exists (n+m). *)
-(*   rewrite /count_sends. rewrite /count_sends in H. rewrite /count_sends in IHn. *)
-(*   rewrite (count_labels_sum _ _ _ _ mtr'); [|done].   *)
-(*   lia. *)
-(* Qed. *)
-
 (* Any fair trace eventually delivers a message *)
-Lemma retransmit_fair_trace_eventually_NDeliver (mtr : mtrace) :
+Lemma retransmit_fair_trace_eventually_Ndeliver (mtr : mtrace) :
   infinite_trace mtr →
   mtrace_valid mtr → mtrace_fair mtr →
   ∃ n, pred_at mtr n (λ st l, l = Some $ inr (Ndeliver,mAB)).
@@ -609,62 +519,6 @@ Proof.
   done.
 Qed.
 
-Fixpoint finite_trace_to_trace {S L} (tr : finite_trace S L) : trace S L :=
-  match tr with
-  | {tr[s]} => ⟨s⟩
-  | tr :tr[ℓ]: s => s -[ℓ]-> (finite_trace_to_trace tr)
-  end.
-
-Definition trace_now {S T} (tr : trace S T) P := pred_at tr 0 P.
-Definition trace_always {S T} (tr : trace S T) P := ∀ n, pred_at tr n P.
-Definition trace_eventually {S T} (tr : trace S T) P := ∃ n, pred_at tr n P.
-Definition trace_until {S T} (tr : trace S T) P Q :=
-  ∃ n, pred_at tr n Q ∧ ∀ m, m < n → pred_at tr m P.
-
-Lemma pred_at_after_is_Some {S T} (tr : trace S T) n P :
-  pred_at tr n P → is_Some $ after n tr.
-Proof. rewrite /pred_at. by case_match. Qed.
-
-Lemma after_is_Some_le {S T} (tr : trace S T) n m :
-  m ≤ n → is_Some $ after n tr → is_Some $ after m tr.
-Proof.
-  revert tr m.
-  induction n; intros tr m Hle.
-  { intros. assert (m = 0) as -> by lia. done. }
-  intros.
-  destruct m; [done|].
-  simpl in *.
-  destruct tr; [done|].
-  apply IHn. lia. done.
-Qed.
-
-Lemma trace_eventually_until {S T} (tr : trace S T) P :
-  trace_eventually tr P → trace_until tr (λ s l, ¬ P s l) P.
-Proof.
-  intros [n Hn].
-  induction n as [n IHn] using lt_wf_ind.
-  assert ((∀ m, m < n → pred_at tr m (λ s l, ¬ P s l)) ∨
-            ¬ (∀ m, m < n → pred_at tr m (λ s l, ¬ P s l))) as [HP|HP];
-    [|by eexists _|].
-  { apply ExcludedMiddle. }
-  eapply not_forall_exists_not in HP as [n' HP].
-  apply Classical_Prop.imply_to_and in HP as [Hlt HP].
-  apply pred_at_neg in HP; last first.
-  { eapply after_is_Some_le; [|by eapply pred_at_after_is_Some]. lia. }
-  eapply pred_at_impl in HP; last first.
-  { intros s l H. apply NNP_P. apply H. }
-  specialize (IHn n' Hlt HP) as [n'' [H' H'']].
-  exists n''. done.
-Qed.
-
-Lemma prefix_trans {A} (l1 l2 l3 : list A) :
-  l1 `prefix_of` l2 → l2 `prefix_of` l3 → l1 `prefix_of` l3.
-Proof. intros [l1' ->] [l2' ->]. by do 2 apply prefix_app_r. Qed.
-
-Lemma suffix_trans {A} (l1 l2 l3 : list A) :
-  l1 `suffix_of` l2 → l2 `suffix_of` l3 → l1 `suffix_of` l3.
-Proof. intros [l1' ->] [l2' ->]. by do 2 apply suffix_app_r. Qed.
-
 Lemma retransmit_fair_trace_buffer_grows (mtr : mtrace) n mtr' :
   mtrace_valid mtr →
   (∀ m, m < n → pred_at mtr m (λ _ l, ¬ option_map label_role l = Some $ inl Brole)) →
@@ -700,7 +554,7 @@ Lemma retransmit_fair_trace_eventually_Received (mtr : mtrace) :
 Proof.
   intros Hafter Htrfirst Hvalid Hfair.
   assert (∃ n, pred_at mtr n (λ st l, l = Some $ inr (Ndeliver,mAB))) as [n Hn].
-  { by apply retransmit_fair_trace_eventually_NDeliver. }
+  { by apply retransmit_fair_trace_eventually_Ndeliver. }
   rewrite /pred_at in Hn.
   apply (infinite_trace_after' n) in Hafter as [mtr' [Hmtr' Hafter]].
   destruct Hfair as [Hfair1 Hfair2].
@@ -783,6 +637,21 @@ Proof.
       destruct H as [? H].
       rewrite H in H6. apply app_eq_nil in H6. set_solver.
     + simpl in *. simplify_eq. destruct t=> /=; simpl in *; simplify_eq; set_solver.
+Qed.
+
+(* A trace starting in the receive role has partially terminated for the Brole *)
+Lemma retransmit_fair_traces_terminate_aux (mtr: mtrace) :
+  (trfirst mtr).1.1 = Received → retransmit_terminating_role (inl Brole) mtr.
+Proof.
+  intros Htrfirst.
+  exists 0. rewrite /pred_at=> /=. simpl in *.
+  destruct mtr as [s|s mtr].
+  - rewrite /pred_at=> /=. simpl in *. destruct s as [[??]?]. simpl in *.
+    simplify_eq. rewrite /retransmit_live_roles. simpl in *.
+    case_decide; set_solver.
+  - rewrite /pred_at=> /=. simpl in *. destruct s as [[??]?]. simpl in *.
+    simplify_eq. rewrite /retransmit_live_roles. simpl in *.
+    case_decide; set_solver.
 Qed.
 
 (* Any fair trace terminates on role B *)
